adjust definition

Specification.thy
@@ -412,10 +412,12 @@ term \<open>valid_unMultigraph.is_Eulerian_trail\<close>
 definition (in valid_graph) is_simple_path :: \<open>_ \<Rightarrow> (_,_) path \<Rightarrow> _ \<Rightarrow> bool\<close> where
   \<open>is_simple_path v ps v' \<longleftrightarrow> is_path v ps v' \<and> distinct (map fst ps)\<close>
 find_theorems "int_vertices"
+definition (in valid_graph) is_trace where \<comment> \<open>non-standard definition. Also not thoroughly thought through.\<close>
+  \<open>is_trace ps \<longleftrightarrow> insert (snd(snd(last ps))) (int_vertices ps) = V\<close>
+definition (in valid_graph) is_hamiltonian_path where
+  \<open>is_hamiltonian_path v ps v' \<longleftrightarrow> is_trace ps \<and> is_simple_path v ps v'\<close>
 definition (in valid_graph) is_hamiltonian where \<comment> \<open>to-do: unconventional intermediate definition, only for experimentation\<close>
   \<open>is_hamiltonian ps \<longleftrightarrow> int_vertices ps = V\<close>
-definition (in valid_graph) is_hamiltonian_path where
-  \<open>is_hamiltonian_path v ps v' \<longleftrightarrow> is_hamiltonian ps \<and> is_simple_path v ps v'\<close>
 
 term "valid_graph.is_path"
 find_theorems \<open>valid_graph.is_path\<close>
@@ -429,8 +431,10 @@ definition \<open>kon_path \<equiv> [(a,ab1,b),(b,bd1,d),(d,cd1,c)]\<close> \<co
 lemma is_simple_path_kon_path: \<open>kon_graph.is_simple_path a kon_path c\<close>
   unfolding kon_graph.is_simple_path_def by (simp add: kon_path_def) (simp add: kon_graph_def)
 
-lemma \<open>kon_graph.is_hamiltonian_path a kon_path b\<close>
-  oops
+lemma \<open>kon_graph.is_hamiltonian_path a kon_path c\<close>
+  apply (simp add: kon_graph.is_hamiltonian_path_def kon_graph.is_trace_def is_simple_path_kon_path)
+  apply eval
+  done
 
 section \<open>Generating Example Input\<close>
 
